New header of horror using IMPORTING

theories/EFSM_LTL.thy
@@ -31,7 +31,7 @@ lemma ltl_step_alt:  "ltl_step e (Some s) r t = (let possibilities = possible_st
                    if possibilities = {||} then (None, [], r)
                    else
                      let (s', t') = Eps (\<lambda>x. x |\<in>| possibilities) in
-                     (Some s', (apply_outputs (Transition.Outputs t') (join_ir (snd t) r)), (apply_updates (Updates t') (join_ir (snd t) r) r))
+                     (Some s', (apply_outputs (Outputs t') (join_ir (snd t) r)), (apply_updates (Updates t') (join_ir (snd t) r) r))
                   )"
   apply (case_tac t)
   by (simp add: Let_def)
@@ -39,75 +39,57 @@ lemma ltl_step_alt:  "ltl_step e (Some s) r t = (let possibilities = possible_st
 primcorec make_full_observation :: "transition_matrix \<Rightarrow> nat option \<Rightarrow> registers \<Rightarrow> event stream \<Rightarrow> state stream" where
   "make_full_observation e s d i = (let (s', o', d') = ltl_step e s d (shd i) in \<lparr>statename = s, datastate = d, event=(shd i), output = o'\<rparr>##(make_full_observation e s' d' (stl i)))"
 
-lemma make_full_observation_unfold: "make_full_observation e s d i = (let (s', o', d') = ltl_step e s d (shd i) in \<lparr>statename = s, datastate = d, event=(shd i), output = o'\<rparr>##(make_full_observation e s' d' (stl i)))"
-  using make_full_observation.code by blast
-
 definition watch :: "transition_matrix \<Rightarrow> event stream \<Rightarrow> state stream" where
   "watch e i \<equiv> (make_full_observation e (Some 0) <> i)"
 
-definition Outputs :: "nat \<Rightarrow> state stream \<Rightarrow> value option" where
-  "Outputs n s \<equiv> nth (output (shd s)) n"
+definition state_eq :: "nat option \<Rightarrow> state stream \<Rightarrow> bool" where
+  "state_eq v s \<equiv> statename (shd s) = v"
 
-definition Inputs :: "nat \<Rightarrow> state stream \<Rightarrow> value" where
-  "Inputs n s \<equiv> nth (inputs (shd s)) (n-1)"
+lemma state_eq_None_not_Some: "state_eq None s \<Longrightarrow> \<not> state_eq (Some n) s"
+  by (simp add: state_eq_def)
 
-definition Registers :: "nat \<Rightarrow> state stream \<Rightarrow> value option" where
-  "Registers n s \<equiv> datastate (shd s) $ n"
+definition label_eq :: "string \<Rightarrow> state stream \<Rightarrow> bool" where
+  "label_eq v s \<equiv> fst (event (shd s)) = (String.implode v)"
 
-definition StateEq :: "nat option \<Rightarrow> state stream \<Rightarrow> bool" where
-  "StateEq v s \<equiv> statename (shd s) = v"
+lemma watch_label: "label_eq l (watch e t) = (fst (shd t) = String.implode l)"
+  by (simp add: label_eq_def watch_def)
 
-lemma StateEq_None_not_Some: "StateEq None s \<Longrightarrow> \<not> StateEq (Some n) s"
-  by (simp add: StateEq_def)
-
-definition LabelEq :: "string \<Rightarrow> state stream \<Rightarrow> bool" where
-  "LabelEq v s \<equiv> fst (event (shd s)) = (String.implode v)"
-
-lemma watch_label: "LabelEq l (watch e t) = (fst (shd t) = String.implode l)"
-  by (simp add: LabelEq_def watch_def)
-
-definition InputEq :: "value list \<Rightarrow> state stream \<Rightarrow> bool" where
-  "InputEq v s \<equiv> inputs (shd s) = v"
+definition input_eq :: "value list \<Rightarrow> state stream \<Rightarrow> bool" where
+  "input_eq v s \<equiv> inputs (shd s) = v"
 
 definition EventEq :: "(string \<times> inputs) \<Rightarrow> state stream \<Rightarrow> bool" where
-  "EventEq e = LabelEq (fst e) aand InputEq (snd e)"
+  "EventEq e = label_eq (fst e) aand input_eq (snd e)"
 
-definition OutputEq :: "value option list \<Rightarrow> state stream \<Rightarrow> bool" where
-  "OutputEq v s \<equiv> output (shd s) = v"
+definition output_eq :: "value option list \<Rightarrow> state stream \<Rightarrow> bool" where
+  "output_eq v s \<equiv> output (shd s) = v"
 
-definition InputLength :: "nat \<Rightarrow> state stream \<Rightarrow> bool" where
-  "InputLength v s \<equiv> length (inputs (shd s)) = v"
+fun check_inx :: "ior \<Rightarrow> nat \<Rightarrow> (value option \<Rightarrow> value option \<Rightarrow> trilean) \<Rightarrow> value option \<Rightarrow> state stream \<Rightarrow> bool" where
+  "check_inx ior.ip n f v s = (f (Some (nth (inputs (shd s)) (n-1))) v = trilean.true)" |
+  "check_inx ior.op n f v s = (f (nth (output (shd s)) n) v = trilean.true)" |
+  "check_inx ior.rg n f v s = (f (datastate (shd s) $ n) v = trilean.true)"
 
-definition OutputLength :: "nat \<Rightarrow> state stream \<Rightarrow> bool" where
-  "OutputLength v s \<equiv> length (output (shd s)) = v"
-
-fun "checkInx" :: "ior \<Rightarrow> nat \<Rightarrow> (value option \<Rightarrow> value option \<Rightarrow> trilean) \<Rightarrow> value option \<Rightarrow> state stream \<Rightarrow> bool" where
-  "checkInx ior.ip n f v s = (f (Some (Inputs (n-1) s)) v = trilean.true)" |
-  "checkInx ior.op n f v s = (f (Outputs n s) v = trilean.true)" |
-  "checkInx ior.rg n f v s = (f (datastate (shd s) $ n) v = trilean.true)"
-
-lemma shd_state_is_none: "(StateEq None) (make_full_observation e None r t)"
-  by (simp add: StateEq_def)
+lemma shd_state_is_none: "(state_eq None) (make_full_observation e None r t)"
+  by (simp add: state_eq_def)
 
 lemma unfold_observe_none: "make_full_observation e None d t = (\<lparr>statename = None, datastate = d, event=(shd t), output = []\<rparr>##(make_full_observation e None d (stl t)))"
   by (simp add: stream.expand)
 
-lemma once_none_always_none: "alw (StateEq None) (make_full_observation e None r t)"
+lemma once_none_always_none: "alw (state_eq None) (make_full_observation e None r t)"
 proof -
   obtain ss :: "((String.literal \<times> value list) stream \<Rightarrow> state stream) \<Rightarrow> (String.literal \<times> value list) stream" where
     "\<forall>f p s. f (stl (ss f)) \<noteq> stl (f (ss f)) \<or> alw p (f s) = alw (\<lambda>s. p (f s)) s"
     by (metis (no_types) alw_inv)
   then show ?thesis
-    by (simp add: StateEq_def all_imp_alw)
+    by (simp add: state_eq_def all_imp_alw)
 qed
 
-lemma no_output_none: "alw (OutputEq []) (make_full_observation e None r t)"
+lemma no_output_none: "alw (output_eq []) (make_full_observation e None r t)"
 proof -
   obtain ss :: "((String.literal \<times> value list) stream \<Rightarrow> state stream) \<Rightarrow> (String.literal \<times> value list) stream" where
     "\<forall>f p s. f (stl (ss f)) \<noteq> stl (f (ss f)) \<or> alw p (f s) = alw (\<lambda>s. p (f s)) s"
     by (metis (no_types) alw_inv)
   then show ?thesis
-    by (simp add: OutputEq_def all_imp_alw)
+    by (simp add: output_eq_def all_imp_alw)
 qed
 
 lemma no_updates_none: "alw (\<lambda>x. datastate (shd x) = r) (make_full_observation e None r t)"
@@ -119,7 +101,7 @@ proof -
     by (simp add: all_imp_alw)
 qed
 
-lemma no_updates_none_individual: "alw (checkInx rg n ValueEq (r $ n)) (make_full_observation e None r t)"
+lemma no_updates_none_individual: "alw (check_inx rg n ValueEq (r $ n)) (make_full_observation e None r t)"
 proof -
   obtain ss :: "((String.literal \<times> value list) stream \<Rightarrow> state stream) \<Rightarrow> (String.literal \<times> value list) stream" where
     "\<forall>f p s. f (stl (ss f)) \<noteq> stl (f (ss f)) \<or> alw p (f s) = alw (\<lambda>s. p (f s)) s"
@@ -128,13 +110,13 @@ proof -
     by (simp add: all_imp_alw)
 qed
 
-lemma event_components: "(LabelEq l aand InputEq i) s = (event (shd s) = (String.implode l, i))"
-  apply (simp add: LabelEq_def InputEq_def)
+lemma event_components: "(label_eq l aand input_eq i) s = (event (shd s) = (String.implode l, i))"
+  apply (simp add: label_eq_def input_eq_def)
   by (metis fst_conv prod.collapse snd_conv)
 
 lemma alw_not_some: "alw (\<lambda>xs. statename (shd xs) \<noteq> Some s) (make_full_observation e None r t)"
   using once_none_always_none[of e r t]
-  unfolding StateEq_def
+  unfolding state_eq_def
   by (simp add: alw_mono)
 
 lemma decompose_pair: "e \<noteq> (l, i) = (\<not> (fst e =l \<and> snd e = i))"
