theories/SAL-examples/Drinks_Machine_LTL.thy
@@ -4,7 +4,7 @@ begin
 
 declare One_nat_def [simp del]
 
-lemma LTL_r2_not_always_gt_100: "not (alw (checkInx rg 2 ValueGt (Some (Num 100)))) (watch drinks i)"
+lemma LTL_r2_not_always_gt_100: "not (alw (check_inx rg 2 ValueGt (Some (Num 100)))) (watch drinks i)"
   apply (simp add: not_alw_iff watch_def)
   apply (rule ev.base)
   by (simp add: ValueGt_def)
@@ -22,7 +22,7 @@ lemma possible_steps_0_not_select: "a \<noteq> STR ''select'' \<Longrightarrow>
   apply safe
   by (simp_all add: select_def)
 
-lemma LTL_nxt_2_means_vend: "alw (nxt (StateEq (Some 2)) impl (StateEq (Some 1))) (watch drinks i)"
+lemma LTL_nxt_2_means_vend: "alw (nxt (state_eq (Some 2)) impl (state_eq (Some 1))) (watch drinks i)"
 proof(coinduction)
   case alw
   then show ?case
@@ -34,31 +34,31 @@ proof(coinduction)
       apply (simp add: possible_steps_0)
       defer
       apply (simp add: possible_steps_select_wrong_arity)
-      apply (metis (no_types, lifting) once_none_always_none StateEq_def alw.cases alw.coinduct option.distinct(1))
+      apply (metis (no_types, lifting) once_none_always_none state_eq_def alw.cases alw.coinduct option.distinct(1))
      apply (simp add: possible_steps_0_not_select)
-     apply (metis (no_types, lifting) once_none_always_none StateEq_def alw.cases alw.coinduct option.distinct(1))
+     apply (metis (no_types, lifting) once_none_always_none state_eq_def alw.cases alw.coinduct option.distinct(1))
     apply standard
-     apply (simp add: StateEq_def)
+     apply (simp add: state_eq_def)
     apply (rule disjI2)
     oops
 
-lemma LTL_costsMoney_aux: "(alw ((not (checkInx rg 2 ValueGt (Some (Num 100)))) impl (not (nxt (StateEq (Some 2)))))) (watch drinks i)"
+lemma LTL_costsMoney_aux: "(alw ((not (check_inx rg 2 ValueGt (Some (Num 100)))) impl (not (nxt (state_eq (Some 2)))))) (watch drinks i)"
   oops
 
   (* costsMoney: THEOREM drinks |- G(X(cfstate=State_2) => gval(value_ge(r_2, Some(NUM(100))))); *)
-lemma LTL_costsMoney: "(alw ((nxt (StateEq (Some 2))) impl ((checkInx rg 2 ValueGt (Some (Num 100)))))) (watch drinks i)"
+lemma LTL_costsMoney: "(alw ((nxt (state_eq (Some 2))) impl ((check_inx rg 2 ValueGt (Some (Num 100)))))) (watch drinks i)"
   oops
 
 (* neverReachS2: THEOREM drinks |- label=select AND I(1) = STR(String_coke) AND
                                 X(label=coin AND I(1) = NUM(100)) AND
                                 X(X(label=vend AND I=InputSequence !empty)) => X(X(X(cfstate=State_2)));;*)
-lemma LTL_neverReachS2:"(((((LabelEq ''select'') aand (checkInx ip 1 ValueEq (Some (Str ''coke''))))
+lemma LTL_neverReachS2:"(((((label_eq ''select'') aand (check_inx ip 1 ValueEq (Some (Str ''coke''))))
                     aand
-                    (nxt ((LabelEq ''coin'') aand (checkInx ip 1 ValueEq (Some (Num 100))))))
+                    (nxt ((label_eq ''coin'') aand (check_inx ip 1 ValueEq (Some (Num 100))))))
                     aand
-                    (nxt (nxt((LabelEq ''vend'' aand (InputEq []))))))
+                    (nxt (nxt((label_eq ''vend'' aand (input_eq []))))))
                     impl
-                    (nxt (nxt (nxt (StateEq (Some 2))))))
+                    (nxt (nxt (nxt (state_eq (Some 2))))))
                     (watch drinks i)"
   oops
 
